latest

experiments/coq-experiments/proplang/Analysis.py
@@ -1,0 +1,50 @@
+import argparse
+from benchtool.Analysis import *
+from benchtool.Plot import *
+from functools import partial
+
+
+def analyze(results: str, images: str):
+    df = parse_results(results)
+
+    if not os.path.exists(images):
+        os.makedirs(images)
+
+    # Generate task bucket charts used in Figure 3.
+    for workload in ['BST']:
+        times = partial(stacked_barchart_times, case=workload, df=df)
+        times(
+            strategies=[
+                'PropLangGenerator',
+                'BespokeGenerator'
+            ],
+            colors=['#000000', '#900D0D', '#DC5F00', '#243763'],
+            limits=[0.001, 0.01, 0.1, 1],
+            limit_type='time',
+            image_path=images,
+            show=False,
+        )
+        times = partial(stacked_barchart_times, case=workload, df=df)
+        times(
+            strategies=[
+                'PropLangGenerator',
+                'BespokeGenerator'
+            ],
+            colors=['#000000', '#900D0D', '#DC5F00', '#243763'],
+            limits=[10, 100, 1000, 10000],
+            limit_type='inputs',
+            image_path=images,
+            show=False,
+
+        )
+
+
+if __name__ == "__main__":
+    p = argparse.ArgumentParser()
+    p.add_argument('--data', help='path to folder for JSON data')
+    p.add_argument('--figures', help='path to folder for figures')
+    args = p.parse_args()
+
+    results_path = f'{os.getcwd()}/{args.data}'
+    images_path = f'{os.getcwd()}/{args.figures}'
+    analyze(results_path, images_path)
