tool/benchtool/Coq.py
@@ -8,46 +8,56 @@ import subprocess
 import ctypes
 import platform
 
-IMPL_DIR = 'Src'
-STRATEGIES_DIR = 'Strategies'
-RUNNERS_DIR = 'Runners'
-SPEC_PATH = 'Src/Spec.v'
+IMPL_DIR = "Src"
+STRATEGIES_DIR = "Strategies"
+RUNNERS_DIR = "Runners"
+SPEC_PATH = "Src/Spec.v"
 
 
 class Coq(BenchTool):
-
-    def __init__(self,
-                 results: str,
-                 log_level: LogLevel = LogLevel.INFO,
-                 replace_level: ReplaceLevel = ReplaceLevel.REPLACE):
+    def __init__(
+        self,
+        results: str,
+        log_level: LogLevel = LogLevel.INFO,
+        replace_level: ReplaceLevel = ReplaceLevel.REPLACE,
+    ):
         super().__init__(
-            Config(start='(*',
-                   end='*)',
-                   ext='.v',
-                   path='workloads/Coq',
-                   ignore='common',
-                   strategies=STRATEGIES_DIR,
-                   impl_path=IMPL_DIR,
-                   spec_path=SPEC_PATH), results, log_level, replace_level)
+            Config(
+                start="(*",
+                end="*)",
+                ext=".v",
+                path="workloads/Coq",
+                ignore="common",
+                strategies=STRATEGIES_DIR,
+                impl_path=IMPL_DIR,
+                spec_path=SPEC_PATH,
+            ),
+            results,
+            log_level,
+            replace_level,
+        )
 
     def all_properties(self, workload: Entry) -> set[str]:
         spec = os.path.join(workload.path, SPEC_PATH)
         with open(spec) as f:
             contents = f.read()
-            regex = re.compile(r'prop_[^\s]*')
+            regex = re.compile(r"prop_[^\s]*")
             matches = regex.findall(contents)
             return list(dict.fromkeys(matches))
 
     def _build(self, workload_path: str):
         strategies = self._get_generator_names(workload_path)
-        strategy_build_commands = map(lambda strategy: self._get_strategy_build_command(strategy),
-                                      strategies)
+        strategy_build_commands = map(
+            lambda strategy: self._get_strategy_build_command(strategy), strategies
+        )
         fuzzers = self._get_fuzzer_names(workload_path)
-        fuzzer_build_commands = map(lambda fuzzer: self._get_fuzzer_build_command(fuzzer), fuzzers)
+        fuzzer_build_commands = map(
+            lambda fuzzer: self._get_fuzzer_build_command(fuzzer), fuzzers
+        )
         with self._change_dir(workload_path):
-            self._shell_command(['coq_makefile', '-f', '_CoqProject', '-o', 'Makefile'])
-            self._shell_command(['make', 'clean'])
-            self._shell_command(['make'])
+            self._shell_command(["coq_makefile", "-f", "_CoqProject", "-o", "Makefile"])
+            self._shell_command(["make", "clean"])
+            self._shell_command(["make"])
 
             for cmd in strategy_build_commands:
                 self._shell_command(cmd.split(" "))
@@ -55,8 +65,12 @@ class Coq(BenchTool):
 
             for i, fuzzer_build_command in enumerate(fuzzer_build_commands):
                 self._log(f"Built fuzzer {fuzzers[i]}", LogLevel.DEBUG)
-                self._log(f"Fuzzer Command 1: {fuzzer_build_command[0]}", LogLevel.DEBUG)
-                self._log(f"Fuzzer Command 2: {fuzzer_build_command[1]}", LogLevel.DEBUG)
+                self._log(
+                    f"Fuzzer Command 1: {fuzzer_build_command[0]}", LogLevel.DEBUG
+                )
+                self._log(
+                    f"Fuzzer Command 2: {fuzzer_build_command[1]}", LogLevel.DEBUG
+                )
                 self._generate_extended_version_of_fuzzer(fuzzers[i])
                 self._shell_command(fuzzer_build_command[2].split(" "))
                 self._shell_command(fuzzer_build_command[3].split(" "))
@@ -72,11 +86,12 @@ class Coq(BenchTool):
 
     def _run_trial_fuzzer(self, workload_path: str, params: TrialArgs):
         with self._change_dir(workload_path):
-            cmd = ['./main_exec', f'./qc_exec {params.property}']
+            cmd = ["./main_exec", f"./qc_exec {params.property}"]
             results = []
             self._log(
                 f"Running {params.workload},{params.strategy},{params.mutant},{params.property}",
-                LogLevel.INFO)
+                LogLevel.INFO,
+            )
             for _ in range(params.trials):
                 try:
                     trial_result = {
@@ -87,21 +102,22 @@ class Coq(BenchTool):
                         "mutant": params.mutant,
                         "passed": None,
                         "property": params.property,
-                        "time": None
+                        "time": None,
                     }
                     process = subprocess.Popen(
-                        cmd,
-                        stdout=subprocess.PIPE,
-                        stderr=subprocess.PIPE,
-                        text=True
+                        cmd, stdout=subprocess.PIPE, stderr=subprocess.PIPE, text=True
                     )
-                    stdout_data, stderr_data = process.communicate(timeout=params.timeout)
+                    stdout_data, stderr_data = process.communicate(
+                        timeout=params.timeout
+                    )
                     start = stdout_data.find("[|")
                     end = stdout_data.find("|]")
 
                     if start == -1 or end == -1:
-                        self._log(f"Unexpected! Error Processing {params.strategy} Output:",
-                                  LogLevel.ERROR)
+                        self._log(
+                            f"Unexpected! Error Processing {params.strategy} Output:",
+                            LogLevel.ERROR,
+                        )
                         self._log(f"[{stdout_data}]", LogLevel.ERROR)
                         self._log(f"[{stderr_data}]", LogLevel.ERROR)
                         trial_result["foundbug"] = False
@@ -109,23 +125,26 @@ class Coq(BenchTool):
                         trial_result["passed"] = 0
                         trial_result["time"] = -1
                     else:
-                        result = stdout_data[start + 2:end]
+                        result = stdout_data[start + 2 : end]
                         self._log(f"{params.strategy} Result: {result}", LogLevel.INFO)
                         json_result = json.loads(result)
                         trial_result["foundbug"] = json_result["result"] in [
-                            "failed", "expected_failure"
+                            "failed",
+                            "expected_failure",
                         ]
                         trial_result["discards"] = json_result["discards"]
                         trial_result["passed"] = json_result["tests"]
-                        trial_result["time"] = float(
-                            json_result["time"]
-                            [:-2]) * 0.001  # ms as string to seconds as float conversion
+                        trial_result["time"] = (
+                            float(json_result["time"][:-2]) * 0.001
+                        )  # ms as string to seconds as float conversion
 
                 except subprocess.TimeoutExpired as e:
                     print(f"Process Timed Out {process.pid}")
                     os.system(f"pkill qc_exec")
                     print(f"Process Output: {e}")
-                    shm_id = int(e.stdout.decode("utf-8").split("|?SHM ID: ")[1].split("?|")[0])
+                    shm_id = int(
+                        e.stdout.decode("utf-8").split("|?SHM ID: ")[1].split("?|")[0]
+                    )
                     print(f"Shared Memory ID: {shm_id}")
                     # Libc is platform dependent, so we need to load it dynamically
                     if platform.system() == "Darwin":
@@ -133,9 +152,13 @@ class Coq(BenchTool):
                     elif platform.system() == "Linux":
                         libc = ctypes.CDLL("libc.so.6")
 
-                    self._log(f"Releasing Shared Memory: {libc.shmctl(int(shm_id), 0, 0)}",
-                              LogLevel.INFO)
-                    self._log(f"Released Shared Memory with ID: {shm_id}", LogLevel.INFO)
+                    self._log(
+                        f"Releasing Shared Memory: {libc.shmctl(int(shm_id), 0, 0)}",
+                        LogLevel.INFO,
+                    )
+                    self._log(
+                        f"Released Shared Memory with ID: {shm_id}", LogLevel.INFO
+                    )
                     trial_result["foundbug"] = False
                     trial_result["discards"] = 0
                     trial_result["passed"] = 0
@@ -152,21 +175,23 @@ class Coq(BenchTool):
                     trial_result["time"] = -1
 
                 results.append(trial_result)
-                if params.short_circuit and trial_result['time'] == params.timeout:
+                if params.short_circuit and trial_result["time"] == params.timeout:
                     break
-                elif trial_result['time'] == -1:
+                elif trial_result["time"] == -1:
                     self._log(f"Exiting due to erroneous trial", LogLevel.ERROR)
                     exit(0)
 
-            json.dump(results, open(params.file, 'w'))
+            json.dump(results, open(params.file, "w"))
 
     def _run_trial_strategy(self, workload_path: str, params: TrialArgs):
         with self._change_dir(workload_path):
+            print(f"{os.getcwd()}")
             cmd = [f"./{params.strategy}_test_runner.native", params.property]
             results = []
             self._log(
                 f"Running {params.workload},{params.strategy},{params.mutant},{params.property}",
-                LogLevel.INFO)
+                LogLevel.INFO,
+            )
             for _ in range(params.trials):
                 trial_result = {
                     "workload": params.workload,
@@ -176,31 +201,28 @@ class Coq(BenchTool):
                     "mutant": params.mutant,
                     "passed": None,
                     "property": params.property,
-                    "time": None
+                    "time": None,
                 }
                 try:
                     process = subprocess.Popen(
-                        cmd,
-                        stdout=subprocess.PIPE,
-                        stderr=subprocess.PIPE,
-                        text=True
+                        cmd, stdout=subprocess.PIPE, stderr=subprocess.PIPE, text=True
                     )
 
-                    stdout_data, stderr_data = process.communicate(timeout=params.timeout)
+                    stdout_data, stderr_data = process.communicate(
+                        timeout=params.timeout
+                    )
 
                     start = stdout_data.find("[|")
                     end = stdout_data.find("|]")
-                    result = stdout_data[start + 2:end]
+                    result = stdout_data[start + 2 : end]
                     self._log(f"{params.strategy} Result: {result}", LogLevel.INFO)
                     json_result = json.loads(result)
-                    trial_result["foundbug"] = json_result["result"] in [
-                        "failed", "expected_failure"
-                    ]
+                    trial_result["foundbug"] = json_result["foundbug"]
                     trial_result["discards"] = json_result["discards"]
-                    trial_result["passed"] = json_result["tests"]
-                    trial_result["time"] = float(
-                        json_result["time"]
-                        [:-2]) * 0.001  # ms as string to seconds as float conversion
+                    trial_result["passed"] = json_result["passed"]
+                    trial_result["time"] = (
+                        float(json_result["time"][:-2]) * 0.001
+                    )  # ms as string to seconds as float conversion
 
                 except subprocess.TimeoutExpired:
                     process.kill()
@@ -212,10 +234,10 @@ class Coq(BenchTool):
                     self._log(f"{params.strategy} Result: Timeout", LogLevel.INFO)
 
                 results.append(trial_result)
-                if params.short_circuit and trial_result['time'] == params.timeout:
+                if params.short_circuit and trial_result["time"] == params.timeout:
                     break
 
-            json.dump(results, open(params.file, 'w'))
+            json.dump(results, open(params.file, "w"))
 
     def _generate_extended_version_of_fuzzer(self, fuzzer: str):
         fuzzer_path = f"./{fuzzer}_test_runner.ml"
@@ -232,7 +254,9 @@ class Coq(BenchTool):
     def _get_executable_strategy_names(self, workload_path):
         strategies_path = f"{workload_path}/{STRATEGIES_DIR}"
         strategies = self._get_strategy_names(strategies_path)
-        executables = list(map(lambda strategy: f"{strategy}_test_runner.native", strategies))
+        executables = list(
+            map(lambda strategy: f"{strategy}_test_runner.native", strategies)
+        )
         return executables
 
     def _get_strategy_build_command(self, strategy: str) -> str:
@@ -240,25 +264,32 @@ class Coq(BenchTool):
         return f"ocamlfind ocamlopt -linkpkg -package zarith -package unix -rectypes {strategy}_test_runner.mli {strategy}_test_runner.ml -o {strategy}_test_runner.native"
 
     def _get_fuzzer_build_command(self, fuzzer: str) -> str:
-        qc_path = os.environ['OPAM_SWITCH_PREFIX'] + '/lib/coq/user-contrib/QuickChick'
+        qc_path = os.environ["OPAM_SWITCH_PREFIX"] + "/lib/coq/user-contrib/QuickChick"
         fuzzer_build_command = (
             f"ocamlfind ocamlopt -ccopt -Wno-error=implicit-function-declaration -afl-instrument -linkpkg -package unix -package str -package coq-core.plugins.extraction -thread -rectypes -w a -o ./qc_exec ./{fuzzer}_test_runner_ext.ml {qc_path}/SHM.c",
             f"ocamlfind ocamlopt -ccopt -Wno-error=implicit-function-declaration -linkpkg -package unix -package str -rectypes -w a -I . -o main_exec {qc_path}/Main.ml {qc_path}/SHM.c",
             f"{qc_path}/cmdprefix.pl {fuzzer}_test_runner_ext.ml",
-            f"{qc_path}/cmdsuffix.pl {fuzzer}_test_runner_ext.ml")
+            f"{qc_path}/cmdsuffix.pl {fuzzer}_test_runner_ext.ml",
+        )
 
         return fuzzer_build_command
 
     def _get_fuzzer_names(self, workload_path):
         fuzzers = list(
-            filter(lambda f: f.endswith("Fuzzer"),
-                   self._get_all_strategy_names(f"{workload_path}/{STRATEGIES_DIR}")))
+            filter(
+                lambda f: f.endswith("Fuzzer"),
+                self._get_all_strategy_names(f"{workload_path}/{STRATEGIES_DIR}"),
+            )
+        )
         return fuzzers
 
     def _get_generator_names(self, workload_path):
         generators = list(
-            filter(lambda f: f.endswith("Generator"),
-                   self._get_all_strategy_names(f"{workload_path}/{STRATEGIES_DIR}")))
+            filter(
+                lambda f: f.endswith("Generator"),
+                self._get_all_strategy_names(f"{workload_path}/{STRATEGIES_DIR}"),
+            )
+        )
         return generators
 
     def _get_all_strategy_names(self, strategies_path) -> list[str]:
@@ -276,26 +307,32 @@ class Coq(BenchTool):
         return self._parse_tests("FuzzChick", s)
 
     def _parse_tests(self, vernacular: str, s: str) -> tuple[list, str]:
-
         def compile(s: str) -> re.Pattern:
             return re.compile(s, flags=re.DOTALL)
 
         start = re.escape(self._config.start)
         end = re.escape(self._config.end)
 
-        test_re = compile(fr"{start}!\s*{vernacular}\s*(\w+).*?{end}")
+        test_re = compile(rf"{start}!\s*{vernacular}\s*(\w+).*?{end}")
         test_ls = re.findall(test_re, s)
+
         return test_ls
 
-    def _generate_test_file_qc(self, runners_path: str, strategy_name: str, tests: list[str],
-                               workload: Entry):
+    def _generate_test_file_parametrized(
+        self,
+        runners_path: str,
+        strategy_name: str,
+        tests: list[str],
+        workload: Entry,
+        test_string_template: str,
+        main_function_string: str,
+    ):
         workload_name = workload.name
         file_name = f"{strategy_name}_test_runner.v"
         strategy_import = f"From {workload_name} Require Import {strategy_name}.\n"
         library_import = "From QuickChick Require Import QuickChick.\n"
         set_warnings = 'Set Warnings "-extraction-opaque-accessed,-extraction".\n'
         size_axiom = 'Axiom num_tests : nat. Extract Constant num_tests => "max_int".\n'
-        test_string_template = "Definition qctest_<test-name> := (fun _ : unit => print_extracted_coq_string (\"[|{\" ++ show (withTime(fun tt => (quickCheckWith (updMaxDiscard (updMaxSuccess (updAnalysis stdArgs true) num_tests) num_tests) <test-name>))) ++ \"}|]\")).\n"
         test_map = f"""
 
 Parameter OCamlString : Type.
@@ -308,14 +345,13 @@ fun test_name ->
   ] in
   let test = List.assoc test_name test_map in
   test ()
-
-
-let () =
-  Sys.argv.(1) |> qctest_map
+{main_function_string}
 ".
 
 """
-        extraction_string_template = f'Extraction "{strategy_name}_test_runner.ml" <test-names> qctest_map.\n'
+        extraction_string_template = (
+            f'Extraction "{strategy_name}_test_runner.ml" <test-names> qctest_map.\n'
+        )
 
         with open(os.path.join(runners_path, file_name), "w") as runner_file:
             runner_file.write(strategy_import)
@@ -327,51 +363,65 @@ let () =
                 runner_file.write(test_string)
             test_names = " ".join(list(map(lambda test: f"qctest_{test}", tests)))
             runner_file.write(test_map)
-            extraction_string = extraction_string_template.replace("<test-names>", test_names)
+            extraction_string = extraction_string_template.replace(
+                "<test-names>", test_names
+            )
             runner_file.write(extraction_string)
 
-    def _generate_test_file_fc(self, runners_path: str, fuzzer_name: str, tests: list[str],
-                               workload: Entry):
-        workload_name = workload.name
-        file_name = f"{fuzzer_name}_test_runner.v"
-        strategy_import = f"From {workload_name} Require Import {fuzzer_name}.\n"
-        library_import = "From QuickChick Require Import QuickChick.\n"
-        set_warnings = 'Set Warnings "-extraction-opaque-accessed,-extraction".\n'
-        test_string_template = "Definition qctest_<test-name> := (fun _ : unit => print_extracted_coq_string (\"[|{\" ++ show (withTime (fun tt => (<test-name>_fuzzer tt))) ++ \"}|]\")).\n"
-        test_map = f"""
+    def _generate_test_file_qc(
+        self, runners_path: str, strategy_name: str, tests: list[str], workload: Entry
+    ):
+        main_function_string = """
+let () =
+  Sys.argv.(1) |> qctest_map
+"""
+        test_string_template = 'Definition qctest_<test-name> := (fun _ : unit => print_extracted_coq_string ("[|{" ++ show (withTime(fun tt => (quickCheckWith (updMaxDiscard (updMaxSuccess (updAnalysis stdArgs true) num_tests) num_tests) <test-name>))) ++ "}|]")).\n'
+        
+        self._generate_test_file_parametrized(
+            runners_path,
+            strategy_name,
+            tests,
+            workload,
+            test_string_template,
+            main_function_string,
+        )
 
-Parameter OCamlString : Type.
-Extract Constant OCamlString => "string".
-Axiom qctest_map : OCamlString -> unit.
-Extract Constant qctest_map => "
-fun test_name ->
-  let test_map = [
-    {'; '.join([f'(""{test_name}"", qctest_{test_name})' for test_name in tests])}
-  ] in
-  let test = List.assoc test_name test_map in
-  test ()
+    def _generate_test_file_pl(
+        self, runners_path: str, strategy_name: str, tests: list[str], workload: Entry
+    ):
+        main_function_string = """
+let () =
+  Sys.argv.(1) |> qctest_map
+"""
+        test_string_template = 'Definition qctest_<test-name> := (fun _ : unit => print_extracted_coq_string ("[|{" ++ show (withTime(fun tt => (sample1 <test-name>))) ++ "}|]")).\n'
+        
+        self._generate_test_file_parametrized(
+            runners_path,
+            strategy_name,
+            tests,
+            workload,
+            test_string_template,
+            main_function_string,
+        )
 
-
+    def _generate_test_file_fc(
+        self, runners_path: str, fuzzer_name: str, tests: list[str], workload: Entry
+    ):
+        main_function_string = """
 let () =
   Printf.printf ""Entering main of qc_exec\\n""; flush stdout;
   setup_shm_aux ();
   Sys.argv.(1) |> qctest_map ; flush stdout;
-".
-
 """
-        extraction_string_template = f'Extraction "{fuzzer_name}_test_runner.ml" <test-names> qctest_map.'
-
-        with open(os.path.join(runners_path, file_name), "w") as runner_file:
-            runner_file.write(strategy_import)
-            runner_file.write(library_import)
-            runner_file.write(set_warnings)
-            for test in tests:
-                test_string = test_string_template.replace("<test-name>", test)
-                runner_file.write(test_string)
-            test_names = " ".join(list(map(lambda test: f"qctest_{test}", tests)))
-            runner_file.write(test_map)
-            extraction_string = extraction_string_template.replace("<test-names>", test_names)
-            runner_file.write(extraction_string)
+        test_string_template = 'Definition qctest_<test-name> := (fun _ : unit => print_extracted_coq_string ("[|{" ++ show (withTime (fun tt => (<test-name>_fuzzer tt))) ++ "}|]")).\n'
+        self._generate_test_file_parametrized(
+            runners_path,
+            fuzzer_name,
+            tests,
+            workload,
+            test_string_template,
+            main_function_string,
+        )
 
     def _preprocess(self, workload: Entry) -> None:
         # Relevant Paths
@@ -381,16 +431,28 @@ let () =
         generators = self._get_generator_names(workload.path)
         fuzzers = self._get_fuzzer_names(workload.path)
         # Empty Runner Directory
-        self._shell_command(['rm', f"{runners_path}*"])
+        self._shell_command(["rm", f"{runners_path}*"])
         # Generate and Add Runners for each strategy
         for strategy in generators:
-            with open(os.path.join(strategies_path, f"{strategy}.v"), "r") as strategy_file:
+            with open(
+                os.path.join(strategies_path, f"{strategy}.v"), "r"
+            ) as strategy_file:
                 content = strategy_file.read()
-                tests = self._parse_tests_qc(content)
-                self._generate_test_file_qc(runners_path, strategy, tests, workload)
+                tests_qc = self._parse_tests_qc(content)
+                tests_pl = self._parse_tests_fc(content)
+                if len(tests_qc) > 0:
+                    self._generate_test_file_qc(
+                        runners_path, strategy, tests_qc, workload
+                    )
+                if len(tests_pl) > 0:
+                    self._generate_test_file_pl(
+                        runners_path, strategy, tests_pl, workload
+                    )
         # Generate and Add Runners for each fuzzer
         for fuzzer in fuzzers:
-            with open(os.path.join(strategies_path, f"{fuzzer}.v"), "r") as strategy_file:
+            with open(
+                os.path.join(strategies_path, f"{fuzzer}.v"), "r"
+            ) as strategy_file:
                 content = strategy_file.read()
                 tests = self._parse_tests_fc(content)
                 self._generate_test_file_fc(runners_path, fuzzer, tests, workload)
@@ -400,9 +462,13 @@ let () =
 
         with open(f"{workload.path}/_CoqProject", "w") as coq_project_file_writer:
             for coq_project_file_line in coq_project_file_contents:
-                if not coq_project_file_line.startswith(
-                        RUNNERS_DIR) and coq_project_file_line != "":
+                if (
+                    not coq_project_file_line.startswith(RUNNERS_DIR)
+                    and coq_project_file_line != ""
+                ):
                     coq_project_file_writer.write(coq_project_file_line + "\n")
 
             for strategy in generators + fuzzers:
-                coq_project_file_writer.write(f"{RUNNERS_DIR}/{strategy}_test_runner.v\n")
+                coq_project_file_writer.write(
+                    f"{RUNNERS_DIR}/{strategy}_test_runner.v\n"
+                )
