workloads/Coq/BST/Src/Impl.v
@@ -20,9 +20,9 @@ Fixpoint insert (k : nat) (v: nat) (t : Tree) :=
   | E => T E k v E
   | T l k' v' r => 
   (*! *)                 
-    (* if k <? k' then T (insert k v l) k' v' r 
+    if k <? k' then T (insert k v l) k' v' r 
     else if k' <? k then T l k' v' (insert k v r) 
-    else T l k' v r *)
+    else T l k' v r
   (*!! insert_1  *)
   (*!
     T E k v E
@@ -34,9 +34,9 @@ Fixpoint insert (k : nat) (v: nat) (t : Tree) :=
  
   (*!! insert_3 *)
   
-  if k <? k' then T (insert k v l) k' v' r
+  (*! if k <? k' then T (insert k v l) k' v' r
   else if k' <? k then T l k' v' (insert k v r)
-  else T l k' v' r
+  else T l k' v' r *)
  
   end.
 
