workloads/Coq/PropLang.v
@@ -1,0 +1,662 @@
+From QuickChick Require Import QuickChick.
+Import QcDefaultNotation. Open Scope qc_scope.
+Set Warnings "-extraction-opaque-accessed,-extraction".
+
+Require Import List ZArith.
+Import ListNotations.
+Import MonadNotation.
+
+Inductive Ctx :=
+| EmptyCtx
+| CtxBind : Type -> Ctx -> Ctx.
+
+Declare Scope prop_scope.
+Notation "'∅'" := EmptyCtx : prop_scope.
+Notation " A '·' C " :=
+  (CtxBind A C) (at level 70) : prop_scope.
+
+Local Open Scope prop_scope.
+
+Fixpoint interpCtx (C : Ctx) : Type :=
+  match C with
+  | ∅ => unit
+  | T·C => T * interpCtx C
+  end.
+
+Notation "'⟦' C '⟧'" := (interpCtx C) : prop_scope.
+
+Inductive CProp : Ctx -> Type -> Type :=
+| ForAll : forall A C F
+      (name: string)
+      (generator : ⟦C⟧ -> G A)
+      (mutator   : ⟦C⟧ -> nat -> A -> G A)
+      (shrinker  : ⟦C⟧ -> A -> list A)
+      (printer   : ⟦C⟧ -> A -> string),
+      CProp (A · C) F -> CProp C F
+| ForAllMaybe : forall A C F
+      (name: string)
+      (generator : ⟦C⟧ -> G (option A))
+      (mutator   : ⟦C⟧ -> nat -> A -> G (option A))
+      (shrinker  : ⟦C⟧ -> A -> list A)
+      (printer   : ⟦C⟧ -> A -> string),
+      CProp (A · C) F -> CProp C F
+  | Predicate : forall C F,
+      (⟦C⟧ -> option bool * F) -> CProp C F.
+
+Fixpoint inputTypes {C : Ctx} {F : Type}
+         (cprop : CProp C F) : Ctx :=
+  match cprop with
+  | ForAll A C _ _ _ _ _ _ cprop' =>
+      A · (inputTypes cprop')
+  | ForAllMaybe A C _ _ _ _ _ _ cprop' =>
+      A · (inputTypes cprop')
+  | Predicate _ _ _ => ∅
+  end.
+
+Fixpoint inputTypesMaybe {C : Ctx} {F : Type}
+         (cprop : CProp C F) : Ctx :=
+  match cprop with
+  | ForAll A C _ _ _ _ _ _ cprop' =>
+      (option A) · (inputTypesMaybe cprop')
+  | ForAllMaybe A C _ _ _ _ _ _ cprop' =>
+      (option A) · (inputTypesMaybe cprop')
+  | Predicate _ _ _ => ∅
+  end.
+
+
+Notation "'⦗' c '⦘'" := (@inputTypes _ _ c).
+Notation "'⟬' c '⟭'" := (@inputTypesMaybe _ _ c).
+
+
+Definition typeHead {C : Ctx} {F : Type}
+         (cprop : CProp C F) : Type :=
+  match cprop with
+  | ForAll A C _ _ _ _ _ _ cprop' => A
+  | ForAllMaybe A C _ _ _ _ _ _ cprop' => A
+  | Predicate _ _ _ => unit
+  end.
+
+
+Definition arb : G nat := choose (0,10).
+Definition gen (n : nat) : G nat := choose (0, n).
+Definition mut (k n : nat) : G nat :=
+  choose (n - k, n + k).
+Definition test (x y : nat) : option bool :=
+  Some (Nat.ltb y x).
+
+Local Open Scope string.
+
+Definition example :=
+  @ForAll _ ∅ _ "x" (fun tt => arb) (fun tt n => mut n) (fun tt n => shrink n) (fun tt n => show n) (
+  @ForAll _ (nat · ∅) _ "y" (fun '(x, tt) => gen x) (fun tt n => mut n) (fun tt n => shrink n) (fun tt n => show n) (
+  @Predicate (nat · (nat · ∅)) unit
+             (fun '(y, (x, tt)) => (test x y, tt)))).
+
+Inductive RunResult {C: Ctx} {F: Type} (cprop : CProp C F) :=
+| Normal : ⟦⦗cprop⦘⟧ -> option bool -> F -> RunResult cprop
+| Discard : ⟦⟬cprop⟭⟧ -> F -> RunResult cprop
+.
+Arguments Normal {C} {F} {cprop}.
+Arguments Discard {C} {F} {cprop}.
+
+Fixpoint genAndRun {C : Ctx} {F : Type}
+         (cprop : CProp C F)
+  : ⟦C⟧ -> G (RunResult cprop) :=
+  match cprop with
+  | ForAll _ _ _ _ gen mut shr pri cprop' =>
+      fun env =>
+        a <- gen env;;
+        res <- genAndRun cprop' (a,env);;
+        match res with
+        | Normal env' truth feedback =>
+            ret (Normal (a,env') truth feedback)
+        | Discard env' feedback =>
+            ret (Discard (Some a, env') feedback)
+        end
+  | Predicate C F prop =>
+      fun env => ret (Some (tt, prop env))
+  end.
+
+Fixpoint justGen {C : Ctx} {F : Type}
+         (cprop : CProp C F)
+  : ⟦C⟧ -> G (⟦⦗cprop⦘⟧) :=
+  match cprop with
+  | ForAll _ _ _ _ gen mut shr pri cprop' =>
+      fun env =>
+        a <- gen env;;
+        env <- justGen cprop' (a,env);;
+        ret (a,env)
+  | Predicate C F prop =>
+      fun env => ret tt
+  end.
+
+Fixpoint mutAll {C : Ctx} {F : Type}
+         (cprop : CProp C F) (t: nat)
+  : ⟦C⟧ -> ⟦⦗cprop⦘⟧ -> (G (⟦⦗cprop⦘⟧)) :=
+  match cprop with
+  | ForAll A C F name gen mut shr pri cprop' =>
+      fun env '(x,xs) =>
+        x' <- mut env t x;;
+        xs' <- mutAll cprop' t (x', env) xs;;
+        ret (x', xs')
+  | Predicate C F prop =>
+      fun _ _ => ret tt
+  end.
+
+Fixpoint mutSome {C : Ctx} {F : Type}
+  (cprop : CProp C F) (t: nat)
+: ⟦C⟧ -> ⟦⦗cprop⦘⟧ -> (G (⟦⦗cprop⦘⟧)) :=
+  match cprop with
+  | ForAll A C F name gen mut shr pri cprop' =>
+    fun env '(x,xs) =>
+    mut_oracle <- choose (0, 1);;
+    x' <- mut env t x;;
+    xs' <- mutSome cprop' t (x', env) xs;;
+    match mut_oracle with
+    | 0 => ret (x', xs')
+    | _ => ret (x, xs')
+    end
+  | Predicate C F prop =>
+  fun _ _ => ret tt
+end.
+
+Fixpoint print {C : Ctx} {F} (cprop : CProp C F)
+  : ⟦C⟧ -> ⟦⦗ cprop ⦘⟧ -> list (string * string) :=
+  match cprop with
+  | ForAll A C F name gen mut shr pr cprop' =>
+      fun env '(a,inps') =>
+        (name, pr env a) :: (print cprop' (a, env) inps')
+  | Predicate C F prop =>
+      fun _ _ => nil
+  end.
+
+Fixpoint showElemList (l: list (string * string)) : string :=
+  match l with
+  | [] => ""
+  | ((k, v) :: []) => (k ++ ": " ++ v) 
+  | ((k, v) :: t) => (k ++ ": " ++ v ++ ", " ++ showElemList t)
+  end.
+
+Local Open Scope Z.
+
+Record Seed {A F: Type} := {
+  input: A;
+  feedback: F;
+  energy: Z;
+}.
+
+Definition mkSeed {A F: Type} (a: A) (f: F) (e: Z): Seed := {| input := a; feedback := f; energy := e |}.
+
+Definition Temperature := Z.
+
+Inductive Directive {A F: Type} :=
+| Generate : Directive
+| Mutate : @Seed A F -> Temperature -> Directive
+.
+
+#[global] Instance showDirective {A F: Type} : Show (@Directive A F) :=
+{|
+  show d := match d with
+            | Generate => "Generate"
+            | Mutate _ t => "Mutate(" ++ show t ++ ")"
+            end
+|}.
+
+
+Class SeedPool {A F Pool: Type} := {
+  (* Creates an empty pool. *)
+  mkPool  : unit -> Pool;
+  (* Adds a useful seed into the pool. *)
+  invest  : (A * F) -> Pool -> Pool;
+  (* Decreases the energy of a seed after a useless trial. *)
+  revise  : Pool -> A -> (A * F) -> Pool;
+  (* Samples the pool for an input. *)
+  sample  : Pool -> @Directive A F;
+  (* Returns the best seed in the pool. *)
+  best    : Pool -> option (@Seed A F);
+}.
+
+
+
+Class Utility {A F Pool: Type} `{SeedPool A F Pool} := {
+  (* Returns true if the feedback is interesting. *)
+  useful  : Pool -> F -> bool;
+  (* Returns a metric of how interesting the feedback is. *)
+  utility : Pool -> F -> Z;
+}.
+
+Class Scalar (A : Type) :=
+  { scale : A -> Z }.
+
+#[global] Instance ScalarZ : Scalar Z :=
+  {| scale := fun x => x |}.
+
+
+(* Class Scheduler {A F Pool: Type} `{SeedPool A F Pool} := {
+  invest  : (A * F) -> Pool -> Pool;
+  revise  : Pool -> A -> (A * F) -> Pool;
+}. *)
+
+Record SingletonPool {A F: Type} := {
+  seed: option (@Seed A F);
+}.
+
+#[global] Instance StaticSingletonPool {A F: Type} `{Dec_Eq A} `{Scalar F} : @SeedPool A F (@SingletonPool A F) :=
+  {| mkPool _ := {| seed := None |};
+     invest seed pool := match seed with 
+                         | (a, f) => {| seed := Some (mkSeed a f 1) |}
+                         end ;
+     revise pool a _ := pool ;
+     sample pool := match seed pool with
+                    | None => Generate
+                    | Some seed => Mutate seed 1
+                    end ;
+     best pool := seed pool
+  |}.
+
+#[global] Instance DynamicMonotonicSingletonPool {A F: Type} `{Dec_Eq A} `{Scalar F} : @SeedPool A F (@SingletonPool A F) :=
+  {| mkPool _ := {| seed := None |};
+    invest seed pool := match seed with 
+                        | (a, f) => {| seed := Some (mkSeed a f 20) |}
+                        end ;
+    revise pool a _ := match seed pool with
+                       | None => pool
+                       | Some seed => 
+                        let a' := input seed in
+                        let f := feedback seed in
+                        let n := energy seed in
+                        if (a = a')? then {| seed := Some (mkSeed a f (n - 1)) |} else pool
+                        end ;               
+    sample pool := match seed pool with
+                   | None => Generate
+                   | Some seed => if (energy seed =? 0) 
+                                    then Generate
+                                    else if (energy seed >? 12) then Mutate seed (energy seed - 12)
+                                    else Mutate seed (13 - energy seed)
+
+                   end ;
+    best pool := seed pool
+|}.
+
+#[global] Instance DynamicResettingSingletonPool {A F: Type} `{Dec_Eq A} `{Scalar F} : @SeedPool A F (@SingletonPool A F) :=
+  {| mkPool _ := {| seed := None |};
+    invest seed pool := match seed with 
+                        | (a, f) => {| seed := Some (mkSeed a f 100) |}
+                        end ;
+    revise pool a _ := match seed pool with
+                       | None => pool
+                       | Some seed => 
+                        let a' := input seed in
+                        let f := feedback seed in
+                        let n := energy seed in
+                        if (a = a')? then {| seed := Some (mkSeed a f (n - 1)) |} else pool
+                        end ;               
+    sample pool := match seed pool with
+                   | None => Generate
+                   | Some seed => if (energy seed =? 0) 
+                                    then Generate
+                                    else if (energy seed >=? 96) then Mutate seed (energy seed - 50)
+                                    else Mutate seed (100 - energy seed)
+                   end ;
+    best pool := match seed pool with
+                 | None => None
+                 | Some seed => if (energy seed =? 0) then None else Some seed
+                 end
+|}.
+
+
+#[global] Instance HillClimbingUtility {A F Pool} `{SeedPool A F Pool} `{Scalar F} 
+: Utility := 
+{|
+  useful  := fun pool feedback' => match best pool with
+                                  | None => true
+                                  | Some seed => (scale feedback') >? (scale (feedback seed))
+                                  end;
+  utility := fun pool feedback' => match best pool with
+                                  | None => scale feedback'
+                                  | Some seed => scale feedback' - (scale (feedback seed))
+                                  end
+|}.
+
+(* 
+Record DoubleQueuePool {A E : Type} := {
+  hpq: list (A * E);
+  lpq: list (A * E);
+}.
+
+Definition insertHighPrioritySeed {A E: Type} (seed: (A * E)) (pool: DoubleQueuePool) : DoubleQueuePool :=
+  {| hpq := (seed :: (hpq pool)) ; lpq := (lpq pool) |}.
+
+Definition insertLowPrioritySeed {A E: Type} (seed: (A * E)) (pool: DoubleQueuePool) : DoubleQueuePool :=
+  {| hpq := (hpq pool) ; lpq := (seed :: (lpq pool)) |} .
+
+Fixpoint maxSeed {A E: Type} `{OrdType E} (cmax: option (A * E)) (q: list (A * E)) : option A :=
+  match q with
+  | [] => match cmax with
+          | None => None
+          | Some (a, e) => Some a
+          end
+  | (h :: t) => match cmax with
+                | None => maxSeed (Some h) t
+                | Some (a, e) => if leq e (snd h) then maxSeed (Some h) t else maxSeed (Some (a, e)) t
+                end
+  end.
+
+Definition sampleSeedDQP {A E : Type} `{OrdType E} (pool: DoubleQueuePool) : option A * DoubleQueuePool :=
+  match (hpq pool) with
+  | []  => (maxSeed None (lpq pool), pool)
+  | _   => (maxSeed None (hpq pool), pool)
+  end.
+
+
+  #[global] Instance SeedPoolDQP {A E : Type} `{OrdType E} : @SeedPool A E (@DoubleQueuePool A E) :=
+  {| mkPool _ := {| hpq := []; lpq := [] |};
+     schedule pool seed := pool;
+     insert seed pool := {| hpq := seed :: (hpq pool); lpq := lpq pool |};
+     sample pool :=
+       match (hpq pool) with
+       | []  => (maxSeed None (lpq pool), pool)
+       | _   => (maxSeed None (hpq pool), pool)
+       end
+  |}. *)
+
+
+
+Fixpoint runAndTest {C:Ctx} {F : Type} (cprop : CProp C F)
+         (cenv : ⟦C⟧)
+         (fenv :  ⟦⦗cprop⦘⟧)
+         {struct cprop}
+  : option bool * F.
+Proof.
+  induction cprop; simpl in *.
+  - destruct fenv as [a fenv'] eqn:H.
+    apply IHcprop.
+    + exact (a, cenv).
+    + exact fenv'.
+  - exact (p cenv).
+Defined.
+
+
+Fixpoint shrinkOnTheFly
+  {C : Ctx} {F: Type}
+  (cprop : CProp C F)
+  (cenv :  ⟦C⟧)
+  (fenv :  ⟦⦗cprop⦘⟧)
+  {struct cprop}
+  : option ⟦⦗cprop⦘⟧.
+Proof.
+  induction cprop; simpl in *.
+  - destruct fenv as [a fenv']. 
+    (* Recurse through the list of shrinks *)
+    induction (shrinker cenv a).
+    (* No more shrinks - try the next element of the property *)
+    + destruct (shrinkOnTheFly _ _ cprop (a,cenv) fenv') eqn:M.
+      * exact (Some (a, i)).
+      * exact None.
+    (* More shrinks - run the property on the shrunk possibility. *)
+    + destruct (runAndTest cprop (a0,cenv) fenv') eqn:T. destruct o.
+      * destruct b.
+        (* Test succeeded - recurse down the list. *)
+        -- apply IHl.
+        (* Test failed - end with current result. *)
+        -- exact (Some (a0, fenv')).     
+      * (* Test discarded - recurse down the list. *)
+        apply IHl.
+  - exact None.
+Defined.
+
+Fixpoint shrinkLoop {F: Type} (fuel : nat)
+  (cprop: CProp ∅ F) (counterexample : ⟦⦗cprop⦘⟧) :
+  ⟦⦗cprop⦘⟧ :=
+  match fuel with
+  | O => counterexample
+  | S fuel' =>
+      match shrinkOnTheFly cprop tt counterexample with
+      | Some c' => shrinkLoop fuel' cprop c'
+      | None => counterexample
+      end
+  end.
+
+Definition generator (cprop: CProp ∅ Z) (directive: @Directive ⟦⦗cprop⦘⟧ Z) :=
+  match directive with
+  | Generate => justGen cprop tt
+  | Mutate seed t => mutAll cprop (Z.to_nat t) tt (input seed)
+  end.
+
+
+Fixpoint runLoop (fuel : nat)
+  (cprop : CProp ∅ Z)
+: G (list (string * string)) :=
+match fuel with
+| O => ret []
+| S fuel' => 
+seed <- justGen cprop tt;;
+let res := runAndTest cprop tt seed in
+let '(truth, feedback) := res in
+  match truth with
+  | Some false =>
+    (* Fails *)
+    let shrinkingResult := shrinkLoop 10 cprop seed in
+    let printingResult := print cprop tt shrinkingResult in
+    ret (("tests to failure", show (200000%nat - fuel)%nat) :: printingResult)
+  | Some true =>
+    (* Passes *)
+    runLoop fuel' cprop
+  | None => 
+    (* Discard *)
+    runLoop fuel' cprop
+  end
+end.
+
+Record Result := {
+ discards: nat;
+ foundbug: bool;
+ passed: nat;
+ counterexample: list (string * string);
+}.
+
+Definition mkResult 
+  (discards: nat)
+  (foundbug: bool)
+  (passed: nat)
+  (counterexample: list (string * string))
+  : Result := {| discards := discards; foundbug := foundbug; passed := passed; counterexample := counterexample |}.
+
+Instance showResult : Show Result :=
+  {| show r := """discards"": " ++ show (discards r) ++
+               ", ""foundbug"": " ++ show (foundbug r) ++
+               ", ""passed"": " ++ show (passed r) ++
+               ", ""counterexample"": """ ++  showElemList (counterexample r) ++ """"
+  |}.
+
+Definition targetLoop
+  (fuel : nat) 
+  (cprop : CProp ∅ Z)
+  {Pool : Type}
+  (seeds : Pool)
+  (poolType: @SeedPool (⟦⦗cprop⦘⟧) Z Pool)
+  (utility: Utility) : G Result :=
+
+  let fix targetLoop' 
+         (fuel : nat) 
+         (passed : nat)
+         (discards: nat)
+         (cprop : CProp ∅ Z)
+         {Pool : Type}
+         (seeds : Pool)
+         (poolType: @SeedPool (⟦⦗cprop⦘⟧) Z Pool)
+         (utility: Utility) : G Result :=
+        match fuel with
+        | O => ret (mkResult discards false passed [])
+        | S fuel' => 
+            let directive := sample seeds in
+            seed <- generator cprop directive;;
+            let res := runAndTest cprop tt seed in
+            let '(truth, feedback) := res in
+            match truth with
+            | Some false =>
+                (* Fails *)
+                let shrinkingResult := shrinkLoop 10 cprop seed in
+                let printingResult := print cprop tt shrinkingResult in
+                ret (mkResult discards true passed printingResult)
+            | Some true =>
+                (* Passes *)
+                match useful seeds feedback with
+                | true =>
+                    let seeds' := invest (seed, feedback) seeds in
+                    targetLoop' fuel' (passed + 1)%nat discards cprop seeds' poolType utility
+                | false =>
+                    let seeds' := match directive with
+                                  | Generate => seeds
+                                  | Mutate source _ => revise seeds (input source) (seed, feedback)
+                                  end in
+                    targetLoop' fuel' (passed + 1)%nat discards cprop seeds' poolType utility
+                end
+            | None => 
+                (* Discard *)
+                targetLoop' fuel' passed (discards + 1)%nat cprop seeds poolType utility
+            end
+        end in
+        targetLoop' fuel 0%nat 0%nat cprop seeds poolType utility.
+
+Definition test2 (x y : nat) : option bool :=
+  Some (negb (Nat.eqb y  x)).
+
+
+Definition example2 :=
+  @ForAll _ ∅ _ "x" (fun tt => arb) (fun tt n => mut n) (fun tt n => shrink n) (fun tt n => show n) (
+  @ForAll _ (nat · ∅) _ "y" (fun '(x, tt) => gen x) (fun tt n => mut n) (fun tt n => shrink n) (fun tt n => show n) (
+  @Predicate (nat · (nat · ∅)) Z
+              (fun '(y, (x, tt)) => (test2 x y, 0)))).
+
+Definition example3 :=
+  @ForAll _ ∅ _ "x" (fun tt => arb) (fun tt n => mut n) (fun tt n => shrink n) (fun tt n => show n) (
+  @ForAll _ (nat · ∅) _ "y" (fun '(x, tt) => gen x) (fun tt n => mut n) (fun tt n => shrink n) (fun tt n => show n) (
+  @Predicate (nat · (nat · ∅)) Z
+              (fun '(y, (x, tt)) => (test2 x y, (2000 - Z.of_nat(x - y) - Z.of_nat(y - x)))))).
+    
+Definition example3' :=
+  forAll arb (fun (x: nat)  =>
+  forAll (gen x) (fun (y: nat)  =>
+  test2 x y)).
+
+
+Definition example4 :=
+  @ForAll _ ∅ _ "x" (fun tt => arb) (fun tt n => mut n) (fun tt n => shrink n) (fun tt n => show n) (
+  @ForAll _ (nat · ∅) _ "y" (fun '(x, tt) => gen x) (fun tt n => mut n) (fun tt n => shrink n) (fun tt n => show n) (
+  @Predicate (nat · (nat · ∅)) Z
+            (fun '(y, (x, tt)) => 
+              let '(res, feedback) := withInstrumentation (fun _ => test2 x y) in
+              (res, Z.of_nat(snd feedback)))
+            )).
+            
+
+#[local] Instance showUnit : Show unit :=
+  {| show _ := "()" |}.
+
+(* Check example3. *)
+(* Check toMonad example3 (3, (2, tt)). *)
+Fixpoint toMonad {C : Ctx} {F: Type} (cprop: CProp C F) : ⟦C⟧ -> Checker :=
+  match cprop with
+  | ForAll A C F name gen mut shr pri cprop' =>
+    fun env =>
+      forAllShrinkShow (gen env) (shr env) (pri env) (fun a => toMonad cprop' (a, env))
+  | Predicate C F prop =>
+    fun env => 
+      forAll (returnGen tt) (fun _ => match prop env with
+                                      | (Some true, _) => returnGen true
+                                      | _ => returnGen false
+                                      end)
+  end.
+
+Definition example3'' := toMonad example3.
+
+(* Sample (targetLoop 1000 example2 (mkPool tt) StaticSingletonPool HillClimbingUtility).
+Sample (targetLoop 1000 example3 (mkPool tt) StaticSingletonPool HillClimbingUtility).
+Sample (targetLoop 1000 example2 (mkPool tt) DynamicSingletonPool HillClimbingUtility).
+Sample (targetLoop 1000 example3 (mkPool tt) DynamicSingletonPool HillClimbingUtility). *)
+
+
+Definition Log := list (string).
+
+Definition printSeed (cprop : CProp ∅ Z ) (seed: @Seed ⟦⦗cprop⦘⟧ Z) : string :=
+   showElemList (print cprop tt (input seed)) ++ ", feedback: " ++ show (feedback seed) ++ ", energy: " ++ show (energy seed).
+
+#[local] Instance showListNL {A: Type} `{Show A} : Show (list A) :=
+  {| show l := String.concat nl (map show l) |}.
+
+
+Fixpoint targetLoopLogged (fuel : nat)
+         (cprop : CProp ∅ Z)
+         {Pool : Type}
+         (seeds : Pool)
+         (poolType: @SeedPool (⟦⦗cprop⦘⟧) Z Pool)
+         (utility: Utility)
+         (log   : Log)
+  : G Log :=
+  match fuel with
+  | O => ret (rev log)
+  | S fuel' => 
+      let directive := sample seeds in
+      seed <- generator cprop directive;;
+      let res := runAndTest cprop tt seed in
+      let '(truth, feedback) := res in
+      let printedSeed := showElemList (print cprop tt seed) in
+      
+      let printedSource := match directive with 
+                           | Generate => "None"
+                           | Mutate seed _ => printSeed cprop seed
+                           end in
+      let log := ("source: [" ++ printedSource ++ "], seed: [" ++ printedSeed ++ ", feedback: " ++ show feedback ++ "], truth: " ++ show truth ++ ", fuel: " ++ show fuel ++ ", directive:" ++ show directive) :: log in
+      match truth with
+      | Some false =>
+          (* Fails *)
+          ret (rev log)
+      | Some true =>
+          (* Passes *)
+          match useful seeds feedback with
+          | true =>
+              let seeds' := invest (seed, feedback) seeds in
+              targetLoopLogged fuel' cprop seeds' poolType utility log
+          | false =>
+              let seeds' := match directive with
+                          | Generate => seeds
+                          | Mutate source _ => revise seeds (input source) (seed, feedback)
+                          end in
+              targetLoopLogged fuel' cprop seeds' poolType utility log
+          end
+      | None => 
+          (* Discard *)
+          targetLoopLogged fuel' cprop seeds poolType utility log
+      end
+  end.
+
+Definition bench_qc := forAll (choose (0, 1000)) (fun tt  => ret (Some true)).
+Definition bench_prl := 
+  @ForAll _ ∅ _ "x" (fun tt => (choose (0, 1000)%nat)) (fun tt n => mut n) (fun tt n => shrink n) (fun tt n => show n) (
+  @Predicate (nat · ∅) Z
+              (fun '(x, tt) => (Some true, 0))).
+
+(* Definition bench_prl_function := (targetLoop 100000 bench_prl (mkPool tt) StaticSingletonPool HillClimbingUtility).
+Definition bench_transformed := toMonad bench_prl tt.
+Definition qctest_bench_qc := (fun _ : unit => print_extracted_coq_string ("[|{" ++ show (withTime(fun tt => (quickCheckWith (updMaxSuccess (updAnalysis stdArgs true) 100000) bench_qc))) ++ "}|]")).
+Definition qctest_bench_prl := (fun _ : unit => print_extracted_coq_string ("[|{" ++ show (withTime(fun tt => (sample1 bench_prl_function))) ++ "}|]")). *)
+
+
+(* Definition qctest_bench_transformed := (fun _ : unit => print_extracted_coq_string ("[|{" ++ show (withTime(fun tt => (quickCheckWith (updMaxSuccess (updAnalysis stdArgs true) 100000) bench_transformed))) ++ "}|]")).
+
+Extraction "bench.ml" qctest_bench_qc qctest_bench_prl qctest_bench_transformed. *)
+
+(* Sample1 (targetLoopLogged 1000 example3 (mkPool tt) StaticSingletonPool HillClimbingUtility nil). *)
+(* Sample1 (targetLoopLogged 1000 example3 (mkPool tt) DynamicResettingSingletonPool HillClimbingUtility nil). *)
+(* Sample1 (targetLoopLogged 1000 example3 (mkPool tt) DynamicMonotonicSingletonPool HillClimbingUtility nil). *)
+Definition test_prop_UnionUnionAssoc_runner := (targetLoopLogged 1000 example4 (mkPool tt) DynamicResettingSingletonPool HillClimbingUtility nil).
+Definition qctest_test_prop_InsertValid := (fun _ : unit => print_extracted_coq_string ("[|{" ++ show (withTime(fun tt => (sample1 test_prop_UnionUnionAssoc_runner))) ++ "}|]")).
+
+Extraction "bench.ml" qctest_test_prop_InsertValid.
+
+(* Sample1 (targetLoop 1000 example3 (mkPool tt) StaticSingletonPool HillClimbingUtility). *)
+
+(* Sample1 (targetLoop 1000 example3 (mkPool tt) StaticSingletonPool HillClimbingUtility).
+Sample1 (targetLoop 1000 example3 (mkPool tt) DynamicMonotonicSingletonPool HillClimbingUtility).
+Sample1 (targetLoop 1000 example3 (mkPool tt) DynamicResettingSingletonPool HillClimbingUtility). *)
